Add proof kernel is subgroup

homomorphism.v
@@ -57,3 +57,36 @@ Proof.
   assumption.
 Qed.
 
+Definition kernel {M M' : Type} (G : group M) (G' : group M') (h : hom M G M' G') : set M :=
+  fun x => hom_f M G M' G' h x = id M' G'.
+Arguments kernel {M M'} G G' h /.
+
+Theorem kernel_has_id : forall {M M' : Type} (G : group M) (G' : group M') (h : hom M G M' G'),
+  belongs (id M G) (kernel G G' h).
+Proof.
+  simpl. intros.
+  apply hom_id_map_id.
+Qed.
+
+Theorem kernel_is_entire : forall {M M' : Type} (G : group M) (G' : group M') (h : hom M G M' G'),
+  forall x y, belongs x (kernel G G' h) -> belongs y (kernel G G' h) -> belongs (bin M G x y) (kernel G G' h).
+Proof.
+  simpl. intros.
+  assert (f_xy_eq_fx_fy := hom_law M G M' G' h x y).
+  rewrite H in f_xy_eq_fx_fy.
+  rewrite H0 in f_xy_eq_fx_fy.
+  rename f_xy_eq_fx_fy into f_xy_eq_id_G'_id_G'.
+
+  rewrite (idR M' G' (id M' G')) in f_xy_eq_id_G'_id_G'.
+  assumption.
+Qed.
+
+Theorem kernel_has_inverse : forall {M M' : Type} (G : group M) (G' : group M') (h : hom M G M' G'),
+  forall x, belongs x (kernel G G' h) -> belongs (inverse M G x) (kernel G G' h).
+Proof.
+  simpl. intros.
+  rewrite (hom_inverse_map_inverse G G' h x).
+  rewrite H.
+  rewrite id_inverse_eq_id.
+  reflexivity.
+Qed.
